swap derivation

std/algo/detailed/Detailed_swap.v
@@ -1,55 +1,51 @@
 From Coq Require Import ssreflect.
 From elpi.apps.derive Require Import derive derive.param2.
 Require Import Hierarchy.
+From Trocq Require Import coverage.
 (* Require Import HoTT_additions Hierarchy. *)
 Unset Uniform Inductive Parameters.
 (* Unset Universe Polymorphism. *)
 Unset Universe Minimization ToSet.
 
-Definition Unit := unit.
+(* Definition Unit := unit. *)
 
-Elpi derive.param2 unit.
-Definition UnitR := unit_R.
-Definition unit_Pred := fun (s1 s2: unit) (RR : unit_R s1 s2)=> unit_R s2 s1.
+Elpi derive.param2 Unit.
+Definition UnitR := Unit_R.
+Definition unit_Pred := fun (s1 s2: Unit) (RR : Unit_R s1 s2)=> Unit_R s2 s1.
 
 Definition unitR_sym : forall u1 u2, UnitR u1 u2 -> UnitR u2 u1.
 Proof.
 move=> u1 u2 uR.
-refine (unit_R_rect unit_Pred _ u1 u2 uR).
-- exact tt_R.
+refine (Unit_R_rect unit_Pred _ u1 u2 uR).
+- exact TT_R.
 Defined.
 
 Definition unitR_symKPred := fun u1 u2 (uR : UnitR u1 u2)=> unitR_sym _ _ (unitR_sym _ _ uR) = uR.
 Definition unitR_symK : forall u1 u2 (uR : UnitR u1 u2), unitR_sym _ _ (unitR_sym _ _ uR) = uR.
 Proof.
 move=> u1 u2 uR.
-refine (unit_R_ind unitR_symKPred _ u1 u2 uR).
+refine (Unit_R_ind unitR_symKPred _ u1 u2 uR).
 exact: eq_refl.
 Defined.
 
-Definition Bool := bool.
-Elpi derive.param2 bool.
-Definition BoolR := bool_R.
+Elpi derive.param2 Bool.
+Definition BoolR := Bool_R.
 
-Notation BoolR_symPred := (fun b1 b2 (bR : bool_R b1 b2)=> bool_R b2 b1).
-Definition boolR_sym : forall b1 b2 (bR : bool_R b1 b2), bool_R b2 b1.
+Notation BoolR_symPred := (fun b1 b2 (bR : Bool_R b1 b2)=> Bool_R b2 b1).
+Definition boolR_sym : forall b1 b2 (bR : Bool_R b1 b2), Bool_R b2 b1.
 Proof.
-refine (fun b1 b2 bR=> bool_R_rect BoolR_symPred _ _ b1 b2 bR).
-- exact: true_R.
-- exact: false_R.
+refine (fun b1 b2 bR=> Bool_R_rect BoolR_symPred _ _ b1 b2 bR).
+- exact: Falseb_R.
+- exact: Trueb_R.
 Defined.
 
-Notation BoolR_symKPred := (fun b1 b2 (bR : bool_R b1 b2)=> boolR_sym _ _ (boolR_sym _ _ bR) = bR).
-Definition boolR_symK : forall b1 b2 (bR : bool_R b1 b2), boolR_sym _ _ (boolR_sym _ _ bR) = bR.
+Notation BoolR_symKPred := (fun b1 b2 (bR : Bool_R b1 b2)=> boolR_sym _ _ (boolR_sym _ _ bR) = bR).
+Definition boolR_symK : forall b1 b2 (bR : Bool_R b1 b2), boolR_sym _ _ (boolR_sym _ _ bR) = bR.
 Proof.
-refine (fun b1 b2 bR=> bool_R_ind BoolR_symKPred _ _ b1 b2 bR).
+refine (fun b1 b2 bR=> Bool_R_ind BoolR_symKPred _ _ b1 b2 bR).
 - exact: eq_refl.
 - exact: eq_refl.
 Defined.
-
-Inductive Wrap : Type :=
-| KWrap1 : unit -> Wrap.
-
 Elpi derive.param2 Wrap.
 Definition WrapR := Wrap_R.
 
@@ -58,7 +54,7 @@ Definition wrapR_sym : forall w1 w2, Wrap_R w1 w2 -> Wrap_R w2 w1.
 Proof.
 refine (fun w1 w2 wR=> Wrap_R_rect wrapR_symPred _ w1 w2 wR).
 refine (fun u1 u2 uR=> _).
-exact: (KWrap1_R _ _ (unitR_sym _ _ uR)).
+exact: (KWrap1_R u2 u1 (unitR_sym u1 u2 uR)).
 Defined.
 
 Notation wrapR_symKPred := (fun w1 w2 (wR : Wrap_R w1 w2) => wrapR_sym _ _ (wrapR_sym _ _ wR) = wR).
@@ -72,18 +68,54 @@ rewrite unitR_symK.
 exact: eq_refl.
 Defined.
 
+Elpi derive.param2 WrapMore.
+Notation wrapMoreR_symPred := (fun w1 w2 (wR : WrapMore_R w1 w2) => WrapMore_R w2 w1).
+Definition wrapMoreR_sym : forall w1 w2, WrapMore_R w1 w2 -> WrapMore_R w2 w1.
+Proof.
+refine (fun w1 w2 wR=> WrapMore_R_rect wrapMoreR_symPred _ _ _ w1 w2 wR).
+- refine (fun u1 u2 uR=> _).
+  refine (fun b1 b2 bR=> _).
+  exact: (KWrap_R u2 u1 (unitR_sym u1 u2 uR) b2 b1 (boolR_sym b1 b2 bR)).
+- refine (fun w1 w2 wR=> _).
+  exact: (KWrapWrap_R w2 w1 (wrapR_sym w1 w2 wR)).
+- refine (fun u1 u2 uR=> _).
+  refine (fun u3 u4 uR2=> _). 
+  refine (fun u5 u6 uR3=> _). 
+  exact: (F_R u2 u1 (unitR_sym u1 u2 uR) u4 u3 (unitR_sym u3 u4 uR2) u6 u5 (unitR_sym u5 u6 uR3)).
+Defined.
+
+Notation wrapMoreR_symKPred := (fun w1 w2 (wR : WrapMore_R w1 w2) => wrapMoreR_sym _ _ (wrapMoreR_sym _ _ wR) = wR).
+Definition WrapMoreR_symK : forall w1 w2 (wR : WrapMore_R w1 w2), wrapMoreR_sym _ _ (wrapMoreR_sym _ _ wR) = wR.
+Proof.
+refine (fun w1 w2 wR=> WrapMore_R_ind wrapMoreR_symKPred _ _ _ w1 w2 wR).
+- refine (fun u1 u2 uR=> _).
+  refine (fun b1 b2 bR=> _).
+  cbn delta beta iota.
+  rewrite unitR_symK boolR_symK.
+  exact: eq_refl.
+- refine (fun w1 w2 wR=> _).
+  cbn delta beta iota.
+  rewrite WrapR_symK.
+  exact: eq_refl.
+- refine (fun u1 u2 uR=> _).
+  refine (fun u3 u4 uR2 => _).
+  refine (fun u5 u6 uR3 => _).
+  cbn delta beta iota.
+  rewrite !unitR_symK. 
+  exact: eq_refl.
+Defined.
 
 Definition Nat := nat.
 Elpi derive.param2 nat.
 Definition NatR := nat_R.
 
 Notation nat_symPred := (fun w1 w2 (wR : nat_R w1 w2) => nat_R w2 w1).
-Definition nat_sym : forall w1 w2, nat_R w1 w2 -> nat_R w2 w1.
+Fixpoint nat_sym : forall w1 w2, nat_R w1 w2 -> nat_R w2 w1.
 Proof.
 refine (fun w1 w2 wR=> nat_R_rect nat_symPred _ _ w1 w2 wR).
 exact: O_R.
 refine (fun n1 n2 nR IH => _).
-exact: S_R.
+apply (S_R _ _ (nat_sym _ _ nR)).
 Defined.
 
 Notation nat_symKPred := (fun w1 w2 (wR : nat_R w1 w2) => nat_sym _ _ (nat_sym _ _ wR) = wR).
@@ -92,7 +124,7 @@ Proof.
 refine (fun w1 w2 wR=> nat_R_ind nat_symKPred _ _ w1 w2 wR).
 exact: eq_refl.
 refine (fun n1 n2 nR IH => _).
-simpl.
+cbn delta beta iota.
 rewrite IH.
 exact: eq_refl.
 Defined.
@@ -100,6 +132,7 @@ Defined.
 Inductive Box (A : Type) : Type := B : A -> Box A.
 Elpi derive.param2 Box.
 
+Check @sym_rel.
 Notation boxR_symPred := (fun A1 A2 (AR: A1 -> A2 -> Type) b1 b2 (bR : Box_R A1 A2 AR b1 b2) => Box_R A2 A1 (sym_rel AR) b2 b1).
 Definition boxR_sym : forall A1 A2 (AR: A1 -> A2 -> Type) b1 b2, Box_R A1 A2 AR b1 b2 -> Box_R A2 A1 (sym_rel AR) b2 b1.
 Proof.
@@ -107,7 +140,8 @@ refine (fun A1 A2 AR=> _).
 refine (fun b1 b2 bR=> _).
 refine (Box_R_rect A1 A2 AR (boxR_symPred A1 A2 AR) _ _ _ bR).
 move=> a1 a2 ar.
-exact: (B_R A2 A1 (sym_rel AR) a2 a1 ar).
+refine (B_R A2 A1 (sym_rel AR) a2 a1 _).
+exact: ( (fun x y r => r) a1 a2 ar).
 Defined.
 
 Notation boxR_symKPred := (fun A1 A2 (AR: A1 -> A2 -> Type) b1 b2 (bR : Box_R A1 A2 AR b1 b2) => boxR_sym A2 A1 (sym_rel AR) b2 b1 (boxR_sym A1 A2 AR b1 b2 bR) = bR).
@@ -153,13 +187,14 @@ Definition List (A : Type) := list A.
 Elpi derive.param2 list.
 
 Notation list_symPred := (fun A1 A2 (AR: A1 -> A2 -> Type) b1 b2 (bR : list_R A1 A2 AR b1 b2) => list_R A2 A1 (sym_rel AR) b2 b1).
-Definition list_sym : forall A1 A2 (AR: A1 -> A2 -> Type) b1 b2, list_R A1 A2 AR b1 b2 -> list_R A2 A1 (sym_rel AR) b2 b1.
+Fixpoint list_sym : forall A1 A2 (AR: A1 -> A2 -> Type) b1 b2, list_R A1 A2 AR b1 b2 -> list_R A2 A1 (sym_rel AR) b2 b1.
 Proof.
 refine (fun A1 A2 AR=> _).
 refine (fun b1 b2 bR=> _).
 refine (list_R_rect A1 A2 AR (list_symPred A1 A2 AR) _ _ _ _ bR).
 - exact: (nil_R A2 A1 (sym_rel AR)).
-- move=> a1 a2 ar l1 l2 lr IH. exact: (cons_R A2 A1 (sym_rel AR) a2 a1 ar l2 l1 IH).
+- move=> a1 a2 ar l1 l2 lr IH. 
+exact: (cons_R A2 A1 (sym_rel AR) a2 a1 ar l2 l1 (list_sym A1 A2 AR _ _ lr)).
 Defined.
 
 Notation list_symKPred := (fun A1 A2 (AR: A1 -> A2 -> Type) b1 b2 (bR : list_R A1 A2 AR b1 b2) => list_sym A2 A1 (sym_rel AR) b2 b1 (list_sym A1 A2 AR b1 b2 bR) = bR).
@@ -171,8 +206,9 @@ refine (fun b1 b2 bR=> _).
 refine (list_R_ind A1 A2 AR (list_symKPred A1 A2 AR) _ _ b1 b2 bR).
 - exact: eq_refl.
 - move=> a1 a2 ar l1 l2 lr IH.
-  simpl. rewrite IH.
-exact: eq_refl.
+  cbn delta beta iota.
+  rewrite IH.
+  exact: eq_refl.
 Defined.
 
 Definition Prod (A B : Type) := prod A B.
