std/algo/tests/test_Rel40.v
@@ -34,3 +34,14 @@ Check ThreeTypes_rel40 : forall A1 A2 AR UR B1 B2 BR BUR C1 C2 CR CUR,  Param40.
 
 Elpi derive List.
 Check List_rel40 : forall A1 A2 AR UR,  Param40.Rel (List A1) (List A2).
+
+From Stdlib Require Import String.
+
+Inductive term := 
+| tRel : nat -> term
+| tVar : string -> term 
+| tApp : term -> term -> term 
+| tLam : term -> term -> term.
+
+
+Elpi derive.param2 list.
